Meta.Decl.Axiom.Choice

coq/ZF/Meta/Test/Axiom/Choice.v
@@ -1,54 +1,17 @@
 Require Import Coq.Lists.List.
 Require Import Coq.Strings.String.
 
-Require Import ZF.Meta.Ctx.
-Require Import ZF.Meta.Term.Decl.
-Require Import ZF.Meta.Env.
-Require Import ZF.Meta.Syntax.
 Require Import ZF.Meta.HasTy.
+Require Import ZF.Meta.Term.HasTyDecl.
+Require Import ZF.Meta.Syntax.
 Require Import ZF.Meta.Ty.
 
 Import ListNotations.
 
-Definition FunctionOn : Decl :=
-  {| para := [TySet; TySet];
-     res  := TyProp;
-     body := HoleT TyProp |}.
+Require Import ZF.Meta.Decl.Axiom.Choice.
 
-Definition empty : Decl :=
-  {| para := [];
-     res  := TySet;
-     body := HoleT TySet |}.
-
-Definition eval : Decl :=
-  {| para := [TySet; TySet];
-     res  := TySet;
-     body := HoleT TySet |}.
-
-Definition env : Env := Env.fromListT
-  [ ("FunctionOn"%string, FunctionOn)
-  ; ("empty"%string     , empty)
-  ; ("eval"%string      , eval)
-  ].
-
-(* forall a,                                                                    *)
-(*  exists f, FunctionOn f a /\ forall x, x :< a -> x <> empty -> eval f x :< x *)
-Definition Choice : Term :=
-  All VarTySet
-    (Ex VarTySet
-      (And
-        (IdentT "FunctionOn" [Var 0; Var 1])
-        (All VarTySet
-          (Imp
-            (Elem (Var 0) (Var 2))
-            (Imp
-              (NotEq (Var 0) (IdentT "empty" []))
-              (Elem (IdentT "eval" [Var 1; Var 0]) (Var 0))))))).
-
-(* The choice example is a proposition in the local test environment.           *)
-Proposition HasTy : HasTyT env Ctx.empty Choice TyProp.
+Proposition Choice : HasTyDeclT (Choice.env) Choice.
 Proof.
-  (* Proof by Hermes + gpt 5.5                                                  *)
   apply HasTyAll, HasTyEx, HasTyAnd.
   - apply HasTyIdentT with (d:=FunctionOn). 1: reflexivity.
     apply HasTyTsCons.
