coq/ZF/Meta/Decl/Axiom/Choice.v
@@ -1,0 +1,47 @@
+Require Import Coq.Lists.List.
+Require Import Coq.Strings.String.
+
+Require Import ZF.Meta.Env.
+Require Import ZF.Meta.Env.
+Require Import ZF.Meta.Syntax.
+Require Import ZF.Meta.Term.Decl.
+Require Import ZF.Meta.Ty.
+
+Import ListNotations.
+
+Require Import ZF.Meta.Decl.Set.Empty.
+Require Import ZF.Meta.Decl.Set.Relation.Eval.
+Require Import ZF.Meta.Decl.Set.Relation.FunctionOn.
+
+Export ZF.Meta.Decl.Set.Empty.
+Export ZF.Meta.Decl.Set.Relation.Eval.
+Export ZF.Meta.Decl.Set.Relation.FunctionOn.
+
+(* forall a,                                                                    *)
+(*  exists f, FunctionOn f a /\ forall x, x :< a -> x <> empty -> eval f x :< x *)
+Definition Choice : DeclT :=
+  {| para := []
+  ;  res  := TyProp
+  ;  body :=
+      All VarTySet
+        (Ex VarTySet
+          (And
+            (IdentT "FunctionOn" [Var 0; Var 1])
+            (All VarTySet
+              (Imp
+                (Elem (Var 0) (Var 2))
+                (Imp
+                  (NotEq (Var 0) (IdentT "empty" []))
+                  (Elem (IdentT "eval" [Var 1; Var 0]) (Var 0)))))))
+  |}.
+
+Definition env : Env := Env.unions
+  [ Env.fromListT
+    [ ("Choice"%string, Choice)
+    ]
+  ; FunctionOn.env
+  ; Empty.env
+  ; Eval.env
+  ].
+
+
