coq/ZF/Meta/Decl/Set/Empty.v
@@ -1,0 +1,22 @@
+Require Import Coq.Lists.List.
+Require Import Coq.Strings.String.
+
+Require Import ZF.Meta.Env.
+Require Import ZF.Meta.Env.
+Require Import ZF.Meta.Syntax.
+Require Import ZF.Meta.Term.Decl.
+Require Import ZF.Meta.Ty.
+
+Import ListNotations.
+
+Definition empty : DeclT :=
+  {| para := [];
+     res  := TySet;
+     body := HoleT TySet |}.
+
+Definition env : Env := Env.unions
+  [ Env.fromListT
+    [ ("empty"%string  , empty)]
+  ].
+
+
