coq/ZF/Meta/Decl/Set/Relation/Eval.v
@@ -1,0 +1,26 @@
+Require Import Coq.Lists.List.
+Require Import Coq.Strings.String.
+
+Require Import ZF.Meta.Env.
+Require Import ZF.Meta.Env.
+Require Import ZF.Meta.Syntax.
+Require Import ZF.Meta.Term.Decl.
+Require Import ZF.Meta.Ty.
+
+Import ListNotations.
+
+Require Import ZF.Meta.Decl.Set.Empty.
+Require Import ZF.Meta.Decl.Set.Relation.FunctionOn.
+
+Definition eval : DeclT :=
+  {| para := [TySet; TySet]
+  ;  res  := TySet
+  ;  body := HoleT TySet
+  |}.
+
+Definition env : Env := Env.unions
+  [ Env.fromListT
+    [ ("eval"%string, eval)]
+  ].
+
+
