coq/ZF/Meta/Decl/Set/Relation/FunctionOn.v
@@ -1,0 +1,21 @@
+Require Import Coq.Lists.List.
+Require Import Coq.Strings.String.
+
+Require Import ZF.Meta.Env.
+Require Import ZF.Meta.Env.
+Require Import ZF.Meta.Syntax.
+Require Import ZF.Meta.Term.Decl.
+Require Import ZF.Meta.Ty.
+
+Import ListNotations.
+
+Definition FunctionOn : DeclT :=
+  {| para := [TySet; TySet];
+     res  := TyProp;
+     body := HoleT TyProp |}.
+
+Definition env : Env := Env.unions
+  [ Env.fromListT
+    [ ("FunctionOn"%string  , FunctionOn)]
+  ].
+
